



Implementations of homogenized behaviours in structural codes : examples and on-going efforts on extending the `MFront` code generator

European Solid Mechanics Conference 2025

Antoine MARTIN

July 2025

The framework

- A maxwellian linear viscoelastic case
- A matrix-inclusion microstructure
- We target the computation at the structure scale

Preliminaries



$$\alpha(\mathbf{x}) = \alpha_c(\mathbf{x}) + \alpha_s(\mathbf{x}) \quad (1)$$

with

$$\begin{aligned} \alpha_c(\mathbf{x}) &= \bar{\alpha} + \Gamma^0(\mathbf{L}_0 : \alpha)(\mathbf{x}) \\ \alpha_s(\mathbf{x}) &= \alpha(\mathbf{x}) - \bar{\alpha} - \Gamma^0(\mathbf{L}_0 : \alpha)(\mathbf{x}) \end{aligned} \quad (2)$$

Non-linear visco-elasticity



$$\begin{aligned}t = 0 : \quad & \sigma(\mathbf{x}, 0) = \sigma_0(\mathbf{x}), \quad \varepsilon(\mathbf{x}, 0) = \varepsilon_0(\mathbf{x}) \\t \geq 0 : \quad & \varepsilon(\mathbf{x}, t) = \bar{\mathbf{E}}(t) + \nabla^S \xi^{\text{per}}(\mathbf{x}, t) \\& \dot{\sigma}(\mathbf{x}, t) = \mathbf{C}(\mathbf{x}) : (\dot{\varepsilon}(\mathbf{x}, t) - f(\sigma(\mathbf{x}, t))) \\& \text{div } \sigma(\mathbf{x}, t) = 0\end{aligned} \tag{3}$$

We follow an implicit resolution :

$$\begin{aligned}\Delta \varepsilon(\mathbf{x}) &= \Delta \bar{\mathbf{E}} + \nabla^S \Delta \xi^{\text{per}}(\mathbf{x}) \\ \Delta \sigma(\mathbf{x}) &= \mathbf{C}(\mathbf{x}) : (\Delta \varepsilon(\mathbf{x}) - \Delta t f(\sigma(\mathbf{x}, t) + \theta \Delta \sigma)) \\ \text{div } \Delta \sigma(\mathbf{x}) &= 0\end{aligned} \tag{4}$$

The maxwellian visco-elasticity



$$\begin{aligned}\Delta\sigma(\mathbf{x}) &= \mathbf{C}(\mathbf{x}) : (\Delta\varepsilon(\mathbf{x}) - \Delta t \mathbf{M}(\mathbf{x}) : (\sigma(\mathbf{x}, t) + \theta \Delta\sigma)) \\ (\mathbf{I} + \theta \Delta t \mathbf{C}(\mathbf{x}) : \mathbf{M}(\mathbf{x})) : \Delta\sigma(\mathbf{x}) &= \mathbf{C}(\mathbf{x}) : (\Delta\varepsilon(\mathbf{x}) - \alpha(\mathbf{x}))\end{aligned}\tag{5}$$

with :

$$\alpha(\mathbf{x}) = \Delta t \mathbf{M}(\mathbf{x}) : \sigma(\mathbf{x}, t)\tag{6}$$

which is

$$\Delta\sigma(\mathbf{x}) = \mathbf{L}(\mathbf{x}) : (\Delta\varepsilon(\mathbf{x}) - \alpha(\mathbf{x}))\tag{7}$$

with

$$\mathbf{L}(\mathbf{x}) = (\mathbf{I} + \theta \Delta t \mathbf{C}(\mathbf{x}) : \mathbf{M}(\mathbf{x}))^{-1} : \mathbf{C}(\mathbf{x})\tag{8}$$

One phase is visco-elastic, the others are purely elastic



One phase is visco-elastic, the others are purely elastic



Sum up and implementation

